Weidenbach_Book/CDCL_W_Partial_Optimal_Model.thy
@@ -18,6 +18,28 @@ lemma (in conflict_driven_clause_learning\<^sub>W_optimal_weight)
 context optimal_encoding
 begin
 
+fun normalize_lit :: \<open>'v literal \<Rightarrow> 'v literal\<close> where
+  \<open>normalize_lit (Pos L) =
+    (if L \<in> replacement_neg ` \<Delta>\<Sigma> then Neg (replacement_pos (SOME K. (K \<in> \<Delta>\<Sigma> \<and> L = replacement_neg K)))
+     else Pos L)\<close> |
+  \<open>normalize_lit (Neg L) =
+    (if L \<in> replacement_neg ` \<Delta>\<Sigma> then Pos (replacement_pos (SOME K. K \<in> \<Delta>\<Sigma> \<and> L = replacement_neg K))
+     else Neg L)\<close>
+
+abbreviation normalize_clause :: \<open>'v clause \<Rightarrow> 'v clause\<close> where
+\<open>normalize_clause C \<equiv> normalize_lit `# C\<close>
+
+lemma normalize_lit_Some_simp[simp]: \<open>(SOME K. K \<in> \<Delta>\<Sigma> \<and> (L\<^sup>\<mapsto>\<^sup>0 = K\<^sup>\<mapsto>\<^sup>0)) = L\<close> if \<open>L \<in> \<Delta>\<Sigma>\<close> for K
+  by (rule some1_equality) (use that in auto)
+
+lemma normalize_lit[simp]:
+  \<open>L \<in> \<Sigma> - \<Delta>\<Sigma> \<Longrightarrow> normalize_lit (Pos L) = (Pos L)\<close>
+  \<open>L \<in> \<Sigma> - \<Delta>\<Sigma> \<Longrightarrow> normalize_lit (Neg L) = (Neg L)\<close>
+  \<open>L \<in> \<Delta>\<Sigma> \<Longrightarrow> normalize_lit (Pos (replacement_neg L)) = Neg (replacement_pos L)\<close>
+  \<open>L \<in> \<Delta>\<Sigma> \<Longrightarrow> normalize_lit (Neg (replacement_neg L)) = Pos (replacement_pos L)\<close>
+  by auto
+
+
 interpretation enc_weight_opt: conflict_driven_clause_learning\<^sub>W_optimal_weight where
   state_eq = state_eq and
   state = state and
@@ -39,853 +61,126 @@ interpretation enc_weight_opt: conflict_driven_clause_learning\<^sub>W_optimal_w
   subgoal using weight_init_state by fast
   done
 
-inductive simple_backtrack_conflict_opt :: \<open>'st \<Rightarrow> 'st \<Rightarrow> bool\<close> where
-  \<open>simple_backtrack_conflict_opt S T\<close>
-  if
-    \<open>backtrack_split (trail S) = (M2, Decided K # M1)\<close> and
-    \<open>negate_ann_lits (trail S) \<in># enc_weight_opt.conflicting_clss S\<close> and
-    \<open>conflicting S = None\<close> and
-    \<open>T \<sim> cons_trail (Propagated (-K) (DECO_clause (trail S)))
-      (add_learned_cls (DECO_clause (trail S)) (reduce_trail_to M1 S))\<close>
-
-inductive_cases simple_backtrack_conflict_optE: \<open>simple_backtrack_conflict_opt S T\<close>
-
-lemma simple_backtrack_conflict_opt_conflict_analysis:
-  assumes \<open>simple_backtrack_conflict_opt S U\<close> and
-    inv: \<open>cdcl\<^sub>W_restart_mset.cdcl\<^sub>W_all_struct_inv (enc_weight_opt.abs_state S)\<close>
-  shows \<open>\<exists>T T'. enc_weight_opt.conflict_opt S T \<and> resolve\<^sup>*\<^sup>* T T'
-    \<and> enc_weight_opt.obacktrack T' U\<close>
-  using assms
-proof (cases rule: simple_backtrack_conflict_opt.cases)
-  case (1 M2 K M1)
-  have tr: \<open>trail S = M2 @ Decided K # M1\<close>
-    using 1 backtrack_split_list_eq[of \<open>trail S\<close>]
-    by auto
-  let ?S = \<open>update_conflicting (Some (negate_ann_lits (trail S))) S\<close>
-  have \<open>enc_weight_opt.conflict_opt S ?S\<close>
-    by (rule enc_weight_opt.conflict_opt.intros[OF 1(2,3)]) auto
-
-  let ?T = \<open>\<lambda>n. update_conflicting
-    (Some (negate_ann_lits (drop n (trail S))))
-    (reduce_trail_to (drop n (trail S)) S)\<close>
-  have proped_M2: \<open>is_proped (M2 ! n)\<close> if \<open>n < length M2\<close> for n
-    using that 1(1) nth_length_takeWhile[of \<open>Not \<circ> is_decided\<close> \<open>trail S\<close>]
-    length_takeWhile_le[of \<open>Not \<circ> is_decided\<close> \<open>trail S\<close>]
-    unfolding backtrack_split_takeWhile_dropWhile
-    apply auto
-    by (metis annotated_lit.exhaust_disc comp_apply nth_mem set_takeWhileD)
-  have is_dec_M2[simp]: \<open>filter_mset is_decided (mset M2) = {#}\<close>
-    using 1(1) nth_length_takeWhile[of \<open>Not \<circ> is_decided\<close> \<open>trail S\<close>]
-    length_takeWhile_le[of \<open>Not \<circ> is_decided\<close> \<open>trail S\<close>]
-    unfolding backtrack_split_takeWhile_dropWhile
-    apply (auto simp: filter_mset_empty_conv)
-    by (metis annotated_lit.exhaust_disc comp_apply nth_mem set_takeWhileD)
-  have n_d: \<open>no_dup (trail S)\<close> and
-    le: \<open>cdcl\<^sub>W_restart_mset.cdcl\<^sub>W_conflicting (enc_weight_opt.abs_state S)\<close> and
-    dist: \<open>cdcl\<^sub>W_restart_mset.distinct_cdcl\<^sub>W_state (enc_weight_opt.abs_state S)\<close> and
-    decomp_imp: \<open>all_decomposition_implies_m (clauses S + (enc_weight_opt.conflicting_clss S))
-      (get_all_ann_decomposition (trail S))\<close> and
-    learned: \<open>cdcl\<^sub>W_restart_mset.cdcl\<^sub>W_learned_clause (enc_weight_opt.abs_state S)\<close>
-    using inv
-    unfolding cdcl\<^sub>W_restart_mset.cdcl\<^sub>W_all_struct_inv_def
-      cdcl\<^sub>W_restart_mset.cdcl\<^sub>W_M_level_inv_def
-    by auto
-  then have [simp]: \<open>K \<noteq> lit_of (M2 ! n)\<close> if \<open>n < length M2\<close> for n
-    using that unfolding tr
-    by (auto simp: defined_lit_nth)
-  have n_d_n: \<open>no_dup (drop n M2 @ Decided K # M1)\<close> for n
-    using n_d unfolding tr
-    by (subst (asm) append_take_drop_id[symmetric, of _ n])
-      (auto simp del: append_take_drop_id dest: no_dup_appendD)
-  have mark_dist: \<open>distinct_mset (mark_of (M2!n))\<close> if \<open>n < length M2\<close> for n
-    using dist that proped_M2[OF that] nth_mem[OF that]
-    unfolding cdcl\<^sub>W_restart_mset.distinct_cdcl\<^sub>W_state_def tr
-    by (cases \<open>M2!n\<close>) (auto simp: tr)
-
-  have [simp]: \<open>undefined_lit (drop n M2) K\<close> for n
-    using n_d defined_lit_mono[of \<open>drop n M2\<close> K M2]
-    unfolding tr
-    by (auto simp: set_drop_subset)
-  from this[of 0] have [simp]: \<open>undefined_lit M2 K\<close>
-    by auto
-  have [simp]: \<open>count_decided (drop n M2) = 0\<close> for n
-    apply (subst count_decided_0_iff)
-    using 1(1) nth_length_takeWhile[of \<open>Not \<circ> is_decided\<close> \<open>trail S\<close>]
-    length_takeWhile_le[of \<open>Not \<circ> is_decided\<close> \<open>trail S\<close>]
-    unfolding backtrack_split_takeWhile_dropWhile
-    by (auto simp: dest!: in_set_dropD set_takeWhileD)
-  from this[of 0] have [simp]: \<open>count_decided M2 = 0\<close> by simp
-  have proped: \<open>\<And>L mark a b.
-      a @ Propagated L mark # b = trail S \<longrightarrow>
-      b \<Turnstile>as CNot (remove1_mset L mark) \<and> L \<in># mark\<close>
-    using le
-    unfolding cdcl\<^sub>W_restart_mset.cdcl\<^sub>W_conflicting_def
-    by auto
-  have mark: \<open>drop (Suc n) M2 @ Decided K # M1 \<Turnstile>as
-      CNot (mark_of (M2 ! n) - unmark (M2 ! n)) \<and>
-      lit_of (M2 ! n) \<in># mark_of (M2 ! n)\<close>
-    if \<open>n < length M2\<close> for n
-    using proped_M2[OF that] that
-      append_take_drop_id[of n M2, unfolded Cons_nth_drop_Suc[OF that, symmetric]]
-      proped[of \<open>take n M2\<close> \<open>lit_of (M2 ! n)\<close> \<open>mark_of (M2 ! n)\<close>
-    \<open>drop (Suc n) M2 @ Decided K # M1\<close>]
-    unfolding tr by (cases \<open>M2!n\<close>) auto
-  have confl: \<open>enc_weight_opt.conflict_opt S ?S\<close>
-    by (rule enc_weight_opt.conflict_opt.intros) (use 1 in auto)
-  have res: \<open>resolve\<^sup>*\<^sup>* ?S (?T n)\<close> if \<open>n \<le> length M2\<close> for n
-    using that unfolding tr
-  proof (induction n)
-    case 0
-    then show ?case
-      using get_all_ann_decomposition_backtrack_split[THEN iffD1, OF 1(1)]
-        1
-      by (cases \<open>get_all_ann_decomposition (trail S)\<close>) (auto simp: tr)
-  next
-    case (Suc n)
-    have [simp]: \<open>\<not> Suc (length M2 - Suc n) < length M2 \<longleftrightarrow> n = 0\<close>
-      using Suc(2) by auto
-    have [simp]: \<open>reduce_trail_to (drop (Suc 0) M2 @ Decided K # M1) S = tl_trail S\<close>
-      apply (subst reduce_trail_to.simps)
-      using Suc by (auto simp: tr )
-    have [simp]: \<open>reduce_trail_to (M2 ! 0 # drop (Suc 0) M2 @ Decided K # M1) S = S\<close>
-      apply (subst reduce_trail_to.simps)
-      using Suc by (auto simp: tr )
-    have [simp]: \<open>(Suc (length M1) -
-          (length M2 - n + (Suc (length M1) - (n - length M2)))) = 0\<close>
-      \<open>(Suc (length M2 + length M1) -
-          (length M2 - n + (Suc (length M1) - (n - length M2)))) =n\<close>
-      \<open>length M2 - n + (Suc (length M1) - (n - length M2)) = Suc (length M2 + length M1) - n\<close>
-      using Suc by auto
-    have [symmetric,simp]: \<open>M2 ! n = Propagated (lit_of (M2 ! n)) (mark_of (M2 ! n))\<close>
-      using Suc proped_M2[of n]
-      by (cases \<open>M2 ! n\<close>)  (auto simp: tr trail_reduce_trail_to_drop hd_drop_conv_nth
-        intro!: resolve.intros)
-    have \<open>- lit_of (M2 ! n) \<in># negate_ann_lits (drop n M2 @ Decided K # M1)\<close>
-      using Suc in_set_dropI[of \<open>n\<close> \<open>map (uminus o lit_of) M2\<close> n]
-      by (simp add: negate_ann_lits_def comp_def drop_map
-         del: nth_mem)
-    moreover have \<open>get_maximum_level (drop n M2 @ Decided K # M1)
-       (remove1_mset (- lit_of (M2 ! n)) (negate_ann_lits (drop n M2 @ Decided K # M1))) =
-      Suc (count_decided M1)\<close>
-      using Suc(2) count_decided_ge_get_maximum_level[of \<open>drop n M2 @ Decided K # M1\<close>
-        \<open>(remove1_mset (- lit_of (M2 ! n)) (negate_ann_lits (drop n M2 @ Decided K # M1)))\<close>]
-      by (auto simp: negate_ann_lits_def tr max_def ac_simps
-        remove1_mset_add_mset_If get_maximum_level_add_mset
-	split: if_splits)
-    moreover have \<open>lit_of (M2 ! n) \<in># mark_of (M2 ! n)\<close>
-      using mark[of n] Suc by auto
-    moreover have \<open>(remove1_mset (- lit_of (M2 ! n))
-         (negate_ann_lits (drop n M2 @ Decided K # M1)) \<union>#
-        (mark_of (M2 ! n) - unmark (M2 ! n))) = negate_ann_lits (drop (Suc n) (trail S))\<close>
-      apply (rule distinct_set_mset_eq)
-      using n_d_n[of n] n_d_n[of \<open>Suc n\<close>] no_dup_distinct_mset[OF n_d_n[of n]] Suc
-        mark[of n] mark_dist[of n]
-      by (auto simp: tr Cons_nth_drop_Suc[symmetric, of n]
-          entails_CNot_negate_ann_lits
-        dest: in_diffD intro: distinct_mset_minus)
-    moreover  { have 1: \<open>(tl_trail
-       (reduce_trail_to (drop n M2 @ Decided K # M1) S)) \<sim>
-	 (reduce_trail_to (drop (Suc n) M2 @ Decided K # M1) S)\<close>
-      apply (subst Cons_nth_drop_Suc[symmetric, of n M2])
-      subgoal using Suc by (auto simp: tl_trail_update_conflicting)
-      subgoal
-        apply (rule state_eq_trans)
-	apply simp
-	apply (cases \<open>length (M2 ! n # drop (Suc n) M2 @ Decided K # M1) < length (trail S)\<close>)
-	apply (auto simp: tl_trail_reduce_trail_to_cons tr)
-	done
-      done
-    have \<open>update_conflicting
-     (Some (negate_ann_lits (drop (Suc n) M2 @ Decided K # M1)))
-     (reduce_trail_to (drop (Suc n) M2 @ Decided K # M1) S) \<sim>
-    update_conflicting
-     (Some (negate_ann_lits (drop (Suc n) M2 @ Decided K # M1)))
-     (tl_trail
-       (update_conflicting (Some (negate_ann_lits (drop n M2 @ Decided K # M1)))
-         (reduce_trail_to (drop n M2 @ Decided K # M1) S)))\<close>
-       apply (rule state_eq_trans)
-       prefer 2
-       apply (rule update_conflicting_state_eq)
-       apply (rule tl_trail_update_conflicting[THEN state_eq_sym[THEN iffD1]])
-       apply (subst state_eq_sym)
-       apply (subst update_conflicting_update_conflicting)
-       apply (rule 1)
-       by fast }
-    ultimately have \<open>resolve (?T n) (?T (n+1))\<close> apply -
-      apply (rule resolve.intros[of _ \<open>lit_of (M2 ! n)\<close> \<open>mark_of (M2 ! n)\<close>])
-      using Suc
-        get_all_ann_decomposition_backtrack_split[THEN iffD1, OF 1(1)] 
-         in_get_all_ann_decomposition_trail_update_trail[of \<open>Decided K\<close> M1 \<open>M2\<close> \<open>S\<close>]
-      by (auto simp: tr trail_reduce_trail_to_drop hd_drop_conv_nth
-        intro!: resolve.intros intro: update_conflicting_state_eq)
-    then show ?case
-      using Suc by (auto simp add: tr)
-  qed
-
-  have \<open>get_maximum_level (Decided K # M1) (DECO_clause M1) = get_maximum_level M1 (DECO_clause M1)\<close>
-    by (rule get_maximum_level_cong)
-      (use n_d in \<open>auto simp: tr get_level_cons_if atm_of_eq_atm_of
-      DECO_clause_def Decided_Propagated_in_iff_in_lits_of_l lits_of_def\<close>)
-  also have \<open>... = count_decided M1\<close>
-    using n_d unfolding tr apply -
-    apply (induction M1 rule: ann_lit_list_induct)
-    subgoal by auto
-    subgoal for L M1'
-      apply (subgoal_tac \<open>\<forall>La\<in>#DECO_clause M1'. get_level (Decided L # M1') La = get_level M1' La\<close>)
-      subgoal
-        using count_decided_ge_get_maximum_level[of \<open>M1'\<close> \<open>DECO_clause M1'\<close>]
-        get_maximum_level_cong[of \<open>DECO_clause M1'\<close> \<open>Decided L # M1'\<close> \<open>M1'\<close>]
-       by (auto simp: get_maximum_level_add_mset tr atm_of_eq_atm_of
-        max_def)
-      subgoal
-        by (auto simp: DECO_clause_def
-          get_level_cons_if atm_of_eq_atm_of Decided_Propagated_in_iff_in_lits_of_l
-          lits_of_def)
-       done
-   subgoal for L C M1'
-      apply (subgoal_tac \<open>\<forall>La\<in>#DECO_clause M1'. get_level (Propagated L C # M1') La = get_level M1' La\<close>)
-      subgoal
-        using count_decided_ge_get_maximum_level[of \<open>M1'\<close> \<open>DECO_clause M1'\<close>]
-        get_maximum_level_cong[of \<open>DECO_clause M1'\<close> \<open>Propagated L C # M1'\<close> \<open>M1'\<close>]
-       by (auto simp: get_maximum_level_add_mset tr atm_of_eq_atm_of
-        max_def)
-      subgoal
-        by (auto simp: DECO_clause_def
-          get_level_cons_if atm_of_eq_atm_of Decided_Propagated_in_iff_in_lits_of_l
-          lits_of_def)
-      done
-    done
-  finally have max: \<open>get_maximum_level (Decided K # M1) (DECO_clause M1) = count_decided M1\<close> .
-  have \<open>trail S \<Turnstile>as CNot (negate_ann_lits (trail S))\<close>
-    by (auto simp: true_annots_true_cls_def_iff_negation_in_model
-      negate_ann_lits_def lits_of_def)
-  then have \<open>clauses S + (enc_weight_opt.conflicting_clss S) \<Turnstile>pm DECO_clause (trail S)\<close>
-     unfolding DECO_clause_def apply -
-    apply (rule all_decomposition_implies_conflict_DECO_clause[OF decomp_imp,
-      of \<open>negate_ann_lits (trail S)\<close>])
-    using 1
-    by auto
-
-  have neg: \<open>trail S \<Turnstile>as CNot (mset (map (uminus o lit_of) (trail S)))\<close>
-    by (auto simp: true_annots_true_cls_def_iff_negation_in_model
-      lits_of_def)
-  have ent: \<open>clauses S + enc_weight_opt.conflicting_clss S \<Turnstile>pm DECO_clause (trail S)\<close>
-    unfolding DECO_clause_def
-    by (rule all_decomposition_implies_conflict_DECO_clause[OF decomp_imp,
-         of \<open>mset (map (uminus o lit_of) (trail S))\<close>])
-      (use neg 1 in \<open>auto simp: negate_ann_lits_def\<close>)
-  have deco: \<open>DECO_clause (M2 @ Decided K # M1) = add_mset (- K) (DECO_clause M1)\<close>
-    by (auto simp: DECO_clause_def)
-  have eg: \<open>reduce_trail_to M1 (reduce_trail_to (Decided K # M1) S) \<sim>
-    reduce_trail_to M1 S\<close>
-    apply (subst reduce_trail_to_compow_tl_trail_le)
-    apply (solves \<open>auto simp: tr\<close>)
-    apply (subst (3)reduce_trail_to_compow_tl_trail_le)
-    apply (solves \<open>auto simp: tr\<close>)
-    apply (auto simp: tr)
-    apply (cases \<open>M2 = []\<close>)
-    apply (auto simp: reduce_trail_to_compow_tl_trail_le reduce_trail_to_compow_tl_trail_eq tr)
-    done
-
-  have U: \<open>cons_trail (Propagated (- K) (DECO_clause (M2 @ Decided K # M1)))
-     (add_learned_cls (DECO_clause (M2 @ Decided K # M1))
-       (reduce_trail_to M1 S)) \<sim>
-    cons_trail (Propagated (- K) (add_mset (- K) (DECO_clause M1)))
-     (reduce_trail_to M1
-       (add_learned_cls (add_mset (- K) (DECO_clause M1))
-         (update_conflicting None
-           (update_conflicting (Some (add_mset (- K) (negate_ann_lits M1)))
-             (reduce_trail_to (Decided K # M1) S)))))\<close>
-    unfolding deco
-    apply (rule cons_trail_state_eq)
-    apply (rule state_eq_trans)
-    prefer 2
-    apply (rule state_eq_sym[THEN iffD1])
-    apply (rule reduce_trail_to_add_learned_cls_state_eq)
-    apply (solves \<open>auto simp: tr\<close>)
-    apply (rule add_learned_cls_state_eq)
-    apply (rule state_eq_trans)
-    prefer 2
-    apply (rule state_eq_sym[THEN iffD1])
-    apply (rule reduce_trail_to_update_conflicting_state_eq)
-    apply (solves \<open>auto simp: tr\<close>)
-    apply (rule state_eq_trans)
-    prefer 2
-    apply (rule state_eq_sym[THEN iffD1])
-    apply (rule update_conflicting_state_eq)
-    apply (rule reduce_trail_to_update_conflicting_state_eq)
-    apply (solves \<open>auto simp: tr\<close>)
-    apply (rule state_eq_trans)
-    prefer 2
-    apply (rule state_eq_sym[THEN iffD1])
-    apply (rule update_conflicting_update_conflicting)
-    apply (rule eg)
-    apply (rule state_eq_trans)
-    prefer 2
-    apply (rule state_eq_sym[THEN iffD1])
-    apply (rule update_conflicting_itself)
-    by (use 1 in auto)
-
-  have bt: \<open>enc_weight_opt.obacktrack (?T (length M2)) U\<close>
-    apply (rule enc_weight_opt.obacktrack.intros[of _ \<open>-K\<close> \<open>negate_ann_lits M1\<close> K M1 \<open>[]\<close>
-      \<open>DECO_clause M1\<close> \<open>count_decided M1\<close>])
-    subgoal by (auto simp: tr)
-    subgoal by (auto simp: tr)
-    subgoal by (auto simp: tr)
-    subgoal
-      using count_decided_ge_get_maximum_level[of \<open>Decided K # M1\<close> \<open>DECO_clause M1\<close>]
-      by (auto simp: tr get_maximum_level_add_mset max_def)
-    subgoal using max by (auto simp: tr)
-    subgoal by (auto simp: tr)
-    subgoal by (auto simp: DECO_clause_def negate_ann_lits_def
-      image_mset_subseteq_mono)
-    subgoal using ent by (auto simp: tr DECO_clause_def)
-    subgoal
-      apply (rule state_eq_trans [OF 1(4)])
-      using 1(4) U by (auto simp: tr)
-    done
-
-  show ?thesis
-    using confl res[of \<open>length M2\<close>, simplified] bt
-    by blast
-qed
-
-inductive conflict_opt0 :: \<open>'st \<Rightarrow> 'st \<Rightarrow> bool\<close> where
-  \<open>conflict_opt0 S T\<close>
-  if
-    \<open>count_decided (trail S) = 0\<close> and
-    \<open>negate_ann_lits (trail S) \<in># enc_weight_opt.conflicting_clss S\<close> and
-    \<open>conflicting S = None\<close> and
-    \<open>T \<sim> update_conflicting (Some {#}) (reduce_trail_to ([] :: ('v, 'v clause) ann_lits) S)\<close>
-
-inductive_cases conflict_opt0E: \<open>conflict_opt0 S T\<close>
-
-inductive cdcl_dpll_bnb_r :: \<open>'st \<Rightarrow> 'st \<Rightarrow> bool\<close> for S :: 'st where
-  cdcl_conflict: "conflict S S' \<Longrightarrow> cdcl_dpll_bnb_r S S'" |
-  cdcl_propagate: "propagate S S' \<Longrightarrow> cdcl_dpll_bnb_r S S'" |
-  cdcl_improve: "enc_weight_opt.improvep S S' \<Longrightarrow> cdcl_dpll_bnb_r S S'" |
-  cdcl_conflict_opt0: "conflict_opt0 S S' \<Longrightarrow> cdcl_dpll_bnb_r S S'" |
-  cdcl_simple_backtrack_conflict_opt:
-    \<open>simple_backtrack_conflict_opt S S' \<Longrightarrow> cdcl_dpll_bnb_r S S'\<close> |
-  cdcl_o': "ocdcl\<^sub>W_o_r S S' \<Longrightarrow> cdcl_dpll_bnb_r S S'"
-
-inductive cdcl_dpll_bnb_r_stgy :: \<open>'st \<Rightarrow> 'st \<Rightarrow> bool\<close> for S :: 'st where
-  cdcl_dpll_bnb_r_conflict: "conflict S S' \<Longrightarrow> cdcl_dpll_bnb_r_stgy S S'" |
-  cdcl_dpll_bnb_r_propagate: "propagate S S' \<Longrightarrow> cdcl_dpll_bnb_r_stgy S S'" |
-  cdcl_dpll_bnb_r_improve: "enc_weight_opt.improvep S S' \<Longrightarrow> cdcl_dpll_bnb_r_stgy S S'" |
-  cdcl_dpll_bnb_r_conflict_opt0: "conflict_opt0 S S' \<Longrightarrow> cdcl_dpll_bnb_r_stgy S S'" |
-  cdcl_dpll_bnb_r_simple_backtrack_conflict_opt:
-    \<open>simple_backtrack_conflict_opt S S' \<Longrightarrow> cdcl_dpll_bnb_r_stgy S S'\<close> |
-  cdcl_dpll_bnb_r_other': "ocdcl\<^sub>W_o_r S S' \<Longrightarrow> no_confl_prop_impr S \<Longrightarrow> cdcl_dpll_bnb_r_stgy S S'"
-
-lemma no_dup_dropI:
-  \<open>no_dup M \<Longrightarrow> no_dup (drop n M)\<close>
-  by (cases \<open>n < length M\<close>)  (auto simp: no_dup_def drop_map[symmetric])
-
-lemma tranclp_resolve_state_eq_compatible:
-  \<open>resolve\<^sup>+\<^sup>+ S T \<Longrightarrow>T \<sim> T' \<Longrightarrow> resolve\<^sup>+\<^sup>+ S T'\<close>
-  apply (induction arbitrary: T' rule: tranclp_induct)
-  apply (auto dest: resolve_state_eq_compatible)
-  by (metis resolve_state_eq_compatible state_eq_ref tranclp_into_rtranclp tranclp_unfold_end)
-
-lemma conflict_opt0_state_eq_compatible:
-  \<open>conflict_opt0 S T \<Longrightarrow> S \<sim> S' \<Longrightarrow> T \<sim> T' \<Longrightarrow> conflict_opt0 S' T'\<close>
-  using state_eq_trans[of T' T
-    \<open>update_conflicting (Some {#}) (reduce_trail_to ([]::('v,'v clause) ann_lits) S)\<close>]
-  using state_eq_trans[of T
-    \<open>update_conflicting (Some {#}) (reduce_trail_to ([]::('v,'v clause) ann_lits) S)\<close>
-    \<open>update_conflicting (Some {#}) (reduce_trail_to ([]::('v,'v clause) ann_lits) S')\<close>]
-  update_conflicting_state_eq[of S S' \<open>Some {#}\<close>]
-  apply (auto simp: conflict_opt0.simps state_eq_sym)
-  using reduce_trail_to_state_eq state_eq_trans update_conflicting_state_eq by blast
-
-
-lemma conflict_opt0_conflict_opt:
-  assumes \<open>conflict_opt0 S U\<close> and
-    inv: \<open>cdcl\<^sub>W_restart_mset.cdcl\<^sub>W_all_struct_inv (enc_weight_opt.abs_state S)\<close>
-  shows \<open>\<exists>T. enc_weight_opt.conflict_opt S T \<and> resolve\<^sup>*\<^sup>* T U\<close>
-proof -
-  have
-    1: \<open>count_decided (trail S) = 0\<close> and
-    neg: \<open>negate_ann_lits (trail S) \<in># enc_weight_opt.conflicting_clss S\<close> and
-    confl: \<open>conflicting S = None\<close> and
-    U: \<open>U \<sim> update_conflicting (Some {#}) (reduce_trail_to ([]::('v,'v clause)ann_lits) S)\<close>
-    using assms by (auto elim: conflict_opt0E)
-  let ?T = \<open>update_conflicting (Some (negate_ann_lits (trail S))) S\<close>
-  have confl: \<open>enc_weight_opt.conflict_opt S ?T\<close>
-    using neg confl
-    by (auto simp: enc_weight_opt.conflict_opt.simps)
-  let ?T = \<open>\<lambda>n. update_conflicting
-    (Some (negate_ann_lits (drop n (trail S))))
-    (reduce_trail_to (drop n (trail S)) S)\<close>
-
-  have proped_M2: \<open>is_proped (trail S ! n)\<close> if \<open>n < length (trail S)\<close> for n
-    using 1 that by (auto simp: count_decided_0_iff is_decided_no_proped_iff)
-  have n_d: \<open>no_dup (trail S)\<close> and
-    le: \<open>cdcl\<^sub>W_restart_mset.cdcl\<^sub>W_conflicting (enc_weight_opt.abs_state S)\<close> and
-    dist: \<open>cdcl\<^sub>W_restart_mset.distinct_cdcl\<^sub>W_state (enc_weight_opt.abs_state S)\<close> and
-    decomp_imp: \<open>all_decomposition_implies_m (clauses S + (enc_weight_opt.conflicting_clss S))
-      (get_all_ann_decomposition (trail S))\<close> and
-    learned: \<open>cdcl\<^sub>W_restart_mset.cdcl\<^sub>W_learned_clause (enc_weight_opt.abs_state S)\<close>
-    using inv
-    unfolding cdcl\<^sub>W_restart_mset.cdcl\<^sub>W_all_struct_inv_def
-      cdcl\<^sub>W_restart_mset.cdcl\<^sub>W_M_level_inv_def
-    by auto
-  have proped: \<open>\<And>L mark a b.
-      a @ Propagated L mark # b = trail S \<longrightarrow>
-      b \<Turnstile>as CNot (remove1_mset L mark) \<and> L \<in># mark\<close>
-    using le
-    unfolding cdcl\<^sub>W_restart_mset.cdcl\<^sub>W_conflicting_def
-    by auto
-  have [simp]: \<open>count_decided (drop n (trail S)) = 0\<close> for n
-    using 1 unfolding count_decided_0_iff
-    by (cases \<open>n < length (trail S)\<close>) (auto dest: in_set_dropD)
-  have [simp]: \<open>get_maximum_level (drop n (trail S)) C = 0\<close> for n C
-    using count_decided_ge_get_maximum_level[of \<open>drop n (trail S)\<close> C]
-    by auto
-  have mark_dist: \<open>distinct_mset (mark_of (trail S!n))\<close> if \<open>n < length (trail S)\<close> for n
-    using dist that proped_M2[OF that] nth_mem[OF that]
-    unfolding cdcl\<^sub>W_restart_mset.distinct_cdcl\<^sub>W_state_def
-    by (cases \<open>trail S!n\<close>) auto
-
-  have res: \<open>resolve (?T n) (?T (Suc n))\<close> if \<open>n < length (trail S)\<close> for n
-  proof -
-    define L and E where
-      \<open>L = lit_of (trail S ! n)\<close> and
-      \<open>E = mark_of (trail S ! n)\<close>
-    have \<open>hd (drop n (trail S)) = Propagated L E\<close> and
-      tr_Sn: \<open>trail S ! n = Propagated L E\<close>
-      using proped_M2[OF that]
-      by (cases \<open>trail S ! n\<close>; auto simp: that hd_drop_conv_nth L_def E_def; fail)+
-    have \<open>L \<in># E\<close> and
-      ent_E: \<open>drop (Suc n) (trail S) \<Turnstile>as CNot (remove1_mset L E)\<close>
-      using proped[of \<open>take n (trail S)\<close> L E \<open>drop (Suc n) (trail S)\<close>]
-        that unfolding tr_Sn[symmetric]
-      by (auto simp: Cons_nth_drop_Suc)
-    have 1: \<open>negate_ann_lits (drop (Suc n) (trail S)) =
-       (remove1_mset (- L) (negate_ann_lits (drop n (trail S))) \<union>#
-        remove1_mset L E)\<close>
-      apply (subst distinct_set_mset_eq_iff[symmetric])
-      subgoal
-        using n_d by (auto simp: no_dup_dropI)
-      subgoal
-        using n_d mark_dist[OF that] unfolding tr_Sn
-        by (auto intro: distinct_mset_mono no_dup_dropI
-	  intro!: distinct_mset_minus)
-      subgoal
-        using ent_E unfolding tr_Sn[symmetric]
-        by (auto simp: negate_ann_lits_def that
-  	    Cons_nth_drop_Suc[symmetric] L_def lits_of_def
-  	    true_annots_true_cls_def_iff_negation_in_model
-	    uminus_lit_swap
-	  dest!: multi_member_split)
-       done
-    have \<open>update_conflicting (Some (negate_ann_lits (drop (Suc n) (trail S))))
-     (reduce_trail_to (drop (Suc n) (trail S)) S) \<sim>
-    update_conflicting
-     (Some
-       (remove1_mset (- L) (negate_ann_lits (drop n (trail S))) \<union>#
-        remove1_mset L E))
-     (tl_trail
-       (update_conflicting (Some (negate_ann_lits (drop n (trail S))))
-         (reduce_trail_to (drop n (trail S)) S)))\<close>
-      unfolding 1[symmetric]
-      apply (rule state_eq_trans)
-      prefer 2
-      apply (rule state_eq_sym[THEN iffD1])
-      apply (rule update_conflicting_state_eq)
-      apply (rule tl_trail_update_conflicting)
-      apply (rule state_eq_trans)
-      prefer 2
-      apply (rule state_eq_sym[THEN iffD1])
-      apply (rule update_conflicting_update_conflicting)
-      apply (rule state_eq_ref)
-      apply (rule update_conflicting_state_eq)
-      using that
-      by (auto simp: reduce_trail_to_compow_tl_trail funpow_swap1)
-    moreover have \<open>L \<in># E\<close>
-      using proped[of \<open>take n (trail S)\<close> L E \<open>drop (Suc n) (trail S)\<close>]
-        that unfolding tr_Sn[symmetric]
-      by (auto simp: Cons_nth_drop_Suc)
-    moreover have \<open>- L \<in># negate_ann_lits (drop n (trail S))\<close>
-      by (auto simp: negate_ann_lits_def L_def
-        in_set_dropI that)
-      term \<open>get_maximum_level (drop n (trail S))\<close>
-    ultimately show ?thesis apply -
-      by (rule resolve.intros[of _ L E])
-        (use that in \<open>auto simp: trail_reduce_trail_to_drop
-	  \<open>hd (drop n (trail S)) = Propagated L E\<close>\<close>)
-  qed
-  have \<open>resolve\<^sup>*\<^sup>* (?T 0) (?T n)\<close> if \<open>n \<le> length (trail S)\<close> for n
-    using that
-    apply (induction n)
-    subgoal by auto
-    subgoal for n
-      using res[of n] by auto
-    done
-  from this[of \<open>length (trail S)\<close>] have \<open>resolve\<^sup>*\<^sup>* (?T 0) (?T (length (trail S)))\<close>
-    by auto
-  moreover have \<open>?T (length (trail S)) \<sim> U\<close>
-    apply (rule state_eq_trans)
-    prefer 2 apply (rule state_eq_sym[THEN iffD1], rule U)
-    by auto
-  moreover have False if \<open>(?T 0) = (?T (length (trail S)))\<close> and \<open>length (trail S) > 0\<close>
-    using arg_cong[OF that(1), of conflicting] that(2)
-    by (auto simp: negate_ann_lits_def)
-  ultimately have \<open>length (trail S) > 0 \<longrightarrow> resolve\<^sup>*\<^sup>* (?T 0) U\<close>
-    using tranclp_resolve_state_eq_compatible[of \<open>?T 0\<close>
-      \<open>?T (length (trail S))\<close> U] apply (subst (asm) rtranclp_unfold)
-    by (auto simp: )
-  then have ?thesis if \<open>length (trail S) > 0\<close>
-    using confl that by auto
-  moreover have ?thesis if \<open>length (trail S) = 0\<close>
-    using that confl U 
-      enc_weight_opt.conflict_opt_state_eq_compatible[of S \<open>(update_conflicting (Some {#}) S)\<close> S U]
-    by (auto simp: state_eq_sym)
-  ultimately show ?thesis
-    by blast
-qed
-
-
-lemma backtrack_split_some_is_decided_then_snd_has_hd2:
-  \<open>\<exists>l\<in>set M. is_decided l \<Longrightarrow> \<exists>M' L' M''. backtrack_split M = (M'', Decided L' # M')\<close>
-  by (metis backtrack_split_snd_hd_decided backtrack_split_some_is_decided_then_snd_has_hd
-    is_decided_def list.distinct(1) list.sel(1) snd_conv)
-
-lemma no_step_conflict_opt0_simple_backtrack_conflict_opt:
-  \<open>no_step conflict_opt0 S \<Longrightarrow> no_step simple_backtrack_conflict_opt S \<Longrightarrow>
-  no_step enc_weight_opt.conflict_opt S\<close>
-  using backtrack_split_some_is_decided_then_snd_has_hd2[of \<open>trail S\<close>]
-    count_decided_0_iff[of \<open>trail S\<close>]
-  by (fastforce simp: conflict_opt0.simps simple_backtrack_conflict_opt.simps
-    enc_weight_opt.conflict_opt.simps
-    annotated_lit.is_decided_def)
-
-lemma no_step_cdcl_dpll_bnb_r_cdcl_bnb_r:
-  assumes \<open>cdcl\<^sub>W_restart_mset.cdcl\<^sub>W_all_struct_inv (enc_weight_opt.abs_state S)\<close>
-  shows
-    \<open>no_step cdcl_dpll_bnb_r S \<longleftrightarrow> no_step cdcl_bnb_r S\<close> (is \<open>?A \<longleftrightarrow> ?B\<close>)
-proof
-  assume ?A
-  show ?B
-    using \<open>?A\<close> no_step_conflict_opt0_simple_backtrack_conflict_opt[of S]
-    by (auto simp: cdcl_bnb_r.simps
-      cdcl_dpll_bnb_r.simps all_conj_distrib)
-next
-  assume ?B
-  show ?A
-    using \<open>?B\<close> simple_backtrack_conflict_opt_conflict_analysis[OF _ assms]
-    by (auto simp: cdcl_bnb_r.simps cdcl_dpll_bnb_r.simps all_conj_distrib assms
-      dest!: conflict_opt0_conflict_opt)
-qed
-
-lemma cdcl_dpll_bnb_r_cdcl_bnb_r:
-  assumes \<open>cdcl_dpll_bnb_r S T\<close> and
-    \<open>cdcl\<^sub>W_restart_mset.cdcl\<^sub>W_all_struct_inv (enc_weight_opt.abs_state S)\<close>
-  shows \<open>cdcl_bnb_r\<^sup>*\<^sup>* S T\<close>
-  using assms
-proof (cases rule: cdcl_dpll_bnb_r.cases)
-  case cdcl_simple_backtrack_conflict_opt
-  then obtain S1 S2 where
-    \<open>enc_weight_opt.conflict_opt S S1\<close>
-    \<open>resolve\<^sup>*\<^sup>* S1 S2\<close> and
-    \<open>enc_weight_opt.obacktrack S2 T\<close>
-    using simple_backtrack_conflict_opt_conflict_analysis[OF _ assms(2), of T]
-    by auto
-  then have \<open>cdcl_bnb_r S S1\<close>
-    \<open>cdcl_bnb_r\<^sup>*\<^sup>* S1 S2\<close>
-    \<open>cdcl_bnb_r S2 T\<close>
-    using  mono_rtranclp[of resolve enc_weight_opt.cdcl_bnb_bj]
-    mono_rtranclp[of enc_weight_opt.cdcl_bnb_bj ocdcl\<^sub>W_o_r]
-    mono_rtranclp[of ocdcl\<^sub>W_o_r cdcl_bnb_r]
-    ocdcl\<^sub>W_o_r.intros enc_weight_opt.cdcl_bnb_bj.resolve
-    cdcl_bnb_r.intros
-    enc_weight_opt.cdcl_bnb_bj.intros
-    by (auto 5 4 dest: cdcl_bnb_r.intros conflict_opt0_conflict_opt)
-  then show ?thesis
-    by auto
-next
-  case cdcl_conflict_opt0
-  then obtain S1 where
-    \<open>enc_weight_opt.conflict_opt S S1\<close>
-    \<open>resolve\<^sup>*\<^sup>* S1 T\<close>
-    using conflict_opt0_conflict_opt[OF _ assms(2), of T]
-    by auto
-  then have \<open>cdcl_bnb_r S S1\<close>
-    \<open>cdcl_bnb_r\<^sup>*\<^sup>* S1 T\<close>
-    using  mono_rtranclp[of resolve enc_weight_opt.cdcl_bnb_bj]
-    mono_rtranclp[of enc_weight_opt.cdcl_bnb_bj ocdcl\<^sub>W_o_r]
-    mono_rtranclp[of ocdcl\<^sub>W_o_r cdcl_bnb_r]
-    ocdcl\<^sub>W_o_r.intros enc_weight_opt.cdcl_bnb_bj.resolve
-    cdcl_bnb_r.intros
-    enc_weight_opt.cdcl_bnb_bj.intros
-    by (auto 5 4 dest: cdcl_bnb_r.intros conflict_opt0_conflict_opt)
-  then show ?thesis
-    by auto
-qed (auto 5 4 dest: cdcl_bnb_r.intros conflict_opt0_conflict_opt simp: assms)
-
-lemma resolve_no_prop_confl: \<open>resolve S T \<Longrightarrow> no_step propagate S \<and> no_step conflict S\<close>
-  by (auto elim!: rulesE )
-lemma cdcl_bnb_r_stgy_res:
-  \<open>resolve S T \<Longrightarrow> cdcl_bnb_r_stgy S T\<close>
-    using enc_weight_opt.cdcl_bnb_bj.resolve[of S T]
-    ocdcl\<^sub>W_o_r.intros[of S T]
-    cdcl_bnb_r_stgy.intros[of S T]
-    resolve_no_prop_confl[of S T]
-  by (auto 5 4 dest: cdcl_bnb_r_stgy.intros conflict_opt0_conflict_opt)
-
-lemma rtranclp_cdcl_bnb_r_stgy_res:
-  \<open>resolve\<^sup>*\<^sup>* S T \<Longrightarrow> cdcl_bnb_r_stgy\<^sup>*\<^sup>* S T\<close>
-    using mono_rtranclp[of resolve cdcl_bnb_r_stgy]
-    cdcl_bnb_r_stgy_res
-  by (auto)
-
-lemma obacktrack_no_prop_confl: \<open>enc_weight_opt.obacktrack S T \<Longrightarrow> no_step propagate S \<and> no_step conflict S\<close>
-  by (auto elim!: rulesE enc_weight_opt.obacktrackE)
-
-lemma cdcl_bnb_r_stgy_bt:
-  \<open>enc_weight_opt.obacktrack S T \<Longrightarrow> cdcl_bnb_r_stgy S T\<close>
-    using enc_weight_opt.cdcl_bnb_bj.backtrack[of S T]
-    ocdcl\<^sub>W_o_r.intros[of S T]
-    cdcl_bnb_r_stgy.intros[of S T]
-    obacktrack_no_prop_confl[of S T]
-  by (auto 5 4 dest: cdcl_bnb_r_stgy.intros conflict_opt0_conflict_opt)
-
-lemma cdcl_dpll_bnb_r_stgy_cdcl_bnb_r_stgy:
-  assumes \<open>cdcl_dpll_bnb_r_stgy S T\<close> and
-    \<open>cdcl\<^sub>W_restart_mset.cdcl\<^sub>W_all_struct_inv (enc_weight_opt.abs_state S)\<close>
-  shows \<open>cdcl_bnb_r_stgy\<^sup>*\<^sup>* S T\<close>
-  using assms
-proof (cases rule: cdcl_dpll_bnb_r_stgy.cases)
-  case cdcl_dpll_bnb_r_simple_backtrack_conflict_opt
-  then obtain S1 S2 where
-    \<open>enc_weight_opt.conflict_opt S S1\<close>
-    \<open>resolve\<^sup>*\<^sup>* S1 S2\<close> and
-    \<open>enc_weight_opt.obacktrack S2 T\<close>
-    using simple_backtrack_conflict_opt_conflict_analysis[OF _ assms(2), of T]
-    by auto
-  then have \<open>cdcl_bnb_r_stgy S S1\<close>
-    \<open>cdcl_bnb_r_stgy\<^sup>*\<^sup>* S1 S2\<close>
-    \<open>cdcl_bnb_r_stgy S2 T\<close>
-    using enc_weight_opt.cdcl_bnb_bj.resolve
-    by (auto dest: cdcl_bnb_r_stgy.intros conflict_opt0_conflict_opt
-      rtranclp_cdcl_bnb_r_stgy_res cdcl_bnb_r_stgy_bt)
-  then show ?thesis
-    by auto
-next
-  case cdcl_dpll_bnb_r_conflict_opt0
-  then obtain S1 where
-    \<open>enc_weight_opt.conflict_opt S S1\<close>
-    \<open>resolve\<^sup>*\<^sup>* S1 T\<close>
-    using conflict_opt0_conflict_opt[OF _ assms(2), of T]
-    by auto
-  then have \<open>cdcl_bnb_r_stgy S S1\<close>
-    \<open>cdcl_bnb_r_stgy\<^sup>*\<^sup>* S1 T\<close>
-    using enc_weight_opt.cdcl_bnb_bj.resolve
-    by (auto dest: cdcl_bnb_r_stgy.intros conflict_opt0_conflict_opt
-      rtranclp_cdcl_bnb_r_stgy_res cdcl_bnb_r_stgy_bt)
-  then show ?thesis
-    by auto
-qed (auto 5 4 dest: cdcl_bnb_r_stgy.intros conflict_opt0_conflict_opt)
-
-lemma cdcl_bnb_r_stgy_cdcl_bnb_r:
-  \<open>cdcl_bnb_r_stgy S T \<Longrightarrow> cdcl_bnb_r S T\<close>
-  by (auto simp: cdcl_bnb_r_stgy.simps cdcl_bnb_r.simps)
-
-lemma rtranclp_cdcl_bnb_r_stgy_cdcl_bnb_r:
-  \<open>cdcl_bnb_r_stgy\<^sup>*\<^sup>* S T \<Longrightarrow> cdcl_bnb_r\<^sup>*\<^sup>* S T\<close>
-  by (induction rule: rtranclp_induct)
-   (auto dest: cdcl_bnb_r_stgy_cdcl_bnb_r)
 
 context
-  fixes S :: 'st
-  assumes S_\<Sigma>: \<open>atms_of_mm (init_clss S) = (\<Sigma> - \<Delta>\<Sigma>) \<union> replacement_pos ` \<Delta>\<Sigma>
-     \<union> replacement_neg ` \<Delta>\<Sigma>\<close>
+  fixes S :: 'st and N :: \<open>'v clauses\<close>
+  assumes S_\<Sigma>: \<open>init_clss S = penc N\<close>
 begin
-lemma cdcl_dpll_bnb_r_stgy_all_struct_inv:
-  \<open>cdcl_dpll_bnb_r_stgy S T \<Longrightarrow> cdcl\<^sub>W_restart_mset.cdcl\<^sub>W_all_struct_inv (enc_weight_opt.abs_state S) \<Longrightarrow>
-    cdcl\<^sub>W_restart_mset.cdcl\<^sub>W_all_struct_inv (enc_weight_opt.abs_state T)\<close>
-  using cdcl_dpll_bnb_r_stgy_cdcl_bnb_r_stgy[of S T]
-    rtranclp_cdcl_bnb_r_all_struct_inv[OF S_\<Sigma>]
-    rtranclp_cdcl_bnb_r_stgy_cdcl_bnb_r[of S T]
-  by auto
-
-end
-
-lemma cdcl_bnb_r_stgy_cdcl_dpll_bnb_r_stgy:
-  \<open>cdcl_bnb_r_stgy S T \<Longrightarrow> \<exists>T. cdcl_dpll_bnb_r_stgy S T\<close>
-  by (meson cdcl_bnb_r_stgy.simps cdcl_dpll_bnb_r_conflict cdcl_dpll_bnb_r_conflict_opt0
-    cdcl_dpll_bnb_r_other' cdcl_dpll_bnb_r_propagate cdcl_dpll_bnb_r_simple_backtrack_conflict_opt
-    cdcl_dpll_bnb_r_stgy.intros(3) no_step_conflict_opt0_simple_backtrack_conflict_opt)
-
-context
-  fixes S :: 'st
-  assumes S_\<Sigma>: \<open>atms_of_mm (init_clss S) = (\<Sigma> - \<Delta>\<Sigma>) \<union> replacement_pos ` \<Delta>\<Sigma>
-     \<union> replacement_neg ` \<Delta>\<Sigma>\<close>
-begin
-
-lemma rtranclp_cdcl_dpll_bnb_r_stgy_cdcl_bnb_r:
-  assumes \<open>cdcl_dpll_bnb_r_stgy\<^sup>*\<^sup>* S T\<close> and
-    \<open>cdcl\<^sub>W_restart_mset.cdcl\<^sub>W_all_struct_inv (enc_weight_opt.abs_state S)\<close>
-  shows \<open>cdcl_bnb_r_stgy\<^sup>*\<^sup>* S T\<close>
-  using assms
-  apply (induction rule: rtranclp_induct)
-  subgoal by auto
-  subgoal for T U
-    using cdcl_dpll_bnb_r_stgy_cdcl_bnb_r_stgy[of T U]
-      rtranclp_cdcl_bnb_r_all_struct_inv[OF S_\<Sigma>, of T]
-      rtranclp_cdcl_bnb_r_stgy_cdcl_bnb_r[of S T]
-    by auto
-  done
-
-lemma rtranclp_cdcl_dpll_bnb_r_stgy_all_struct_inv:
-  \<open>cdcl_dpll_bnb_r_stgy\<^sup>*\<^sup>* S T \<Longrightarrow> cdcl\<^sub>W_restart_mset.cdcl\<^sub>W_all_struct_inv (enc_weight_opt.abs_state S) \<Longrightarrow>
-    cdcl\<^sub>W_restart_mset.cdcl\<^sub>W_all_struct_inv (enc_weight_opt.abs_state T)\<close>
-  using rtranclp_cdcl_dpll_bnb_r_stgy_cdcl_bnb_r[of T]
-    rtranclp_cdcl_bnb_r_all_struct_inv[OF S_\<Sigma>, of T]
-    rtranclp_cdcl_bnb_r_stgy_cdcl_bnb_r[of S T]
-  by auto
-
-lemma full_cdcl_dpll_bnb_r_stgy_full_cdcl_bnb_r_stgy:
-  assumes \<open>full cdcl_dpll_bnb_r_stgy S T\<close> and
-    \<open>cdcl\<^sub>W_restart_mset.cdcl\<^sub>W_all_struct_inv (enc_weight_opt.abs_state S)\<close>
-  shows \<open>full cdcl_bnb_r_stgy S T\<close>
-  using no_step_cdcl_dpll_bnb_r_cdcl_bnb_r[of T]
-    rtranclp_cdcl_dpll_bnb_r_stgy_cdcl_bnb_r[of T]
-    rtranclp_cdcl_dpll_bnb_r_stgy_all_struct_inv[of T] assms
-      rtranclp_cdcl_bnb_r_stgy_cdcl_bnb_r[of S T]
-  by (auto simp: full_def
-    dest: cdcl_bnb_r_stgy_cdcl_bnb_r cdcl_bnb_r_stgy_cdcl_dpll_bnb_r_stgy)
-
-end
-
-definition lonely_lit_in_add_only :: \<open>'st \<Rightarrow> bool\<close> where
-\<open>lonely_lit_in_add_only S \<longleftrightarrow>
-  (\<forall>L C. L \<in> \<Delta>\<Sigma> \<longrightarrow> C \<in># clauses S \<longrightarrow> L \<in> atms_of C \<longrightarrow> C \<in># additional_constraint L) \<and>
-  (\<forall>L. L \<in> \<Delta>\<Sigma> \<longrightarrow> conflicting S \<noteq> None \<longrightarrow> L \<in> atms_of (the (conflicting S)) \<longrightarrow>
-    the (conflicting S) \<in># additional_constraint L)\<close>
-
-definition lonely_not_decided :: \<open>'st \<Rightarrow> bool\<close> where
-\<open>lonely_not_decided S \<longleftrightarrow>
-  (\<forall>L. atm_of L \<in> \<Delta>\<Sigma> \<longrightarrow> Decided L \<notin> set (trail S))\<close>
-
-(*TODO Move*)
-lemma backtrack_split_get_all_ann_decompositionD:
-  \<open>backtrack_split M = (a, b) \<Longrightarrow> (b, a) \<in> set (get_all_ann_decomposition M)\<close>
-  using get_all_ann_decomposition_backtrack_split[of M a b]
-  by (cases \<open>get_all_ann_decomposition M\<close>) auto
-
-lemma cdcl_dpll_bnb_r_lonely_not_decided:
-  assumes \<open>cdcl_dpll_bnb_r S T\<close> and
-    \<open>lonely_not_decided S\<close>
-  shows \<open>lonely_not_decided T\<close>
-  using assms
-  by (induction)
-    (auto simp: conflict.simps lonely_not_decided_def
-       ocdcl\<^sub>W_o_r.simps enc_weight_opt.cdcl_bnb_bj.simps
-     elim!: rulesE enc_weight_opt.improveE conflict_opt0E
-       simple_backtrack_conflict_optE odecideE
-       enc_weight_opt.obacktrackE
-     dest!: backtrack_split_get_all_ann_decompositionD in_set_tlD)
 
 lemma
   assumes
-    \<open>cdcl_dpll_bnb_r S T\<close> and
-    lone: \<open>lonely_lit_in_add_only S\<close> and
-    ndec: \<open>lonely_not_decided S\<close>
-  shows \<open>lonely_lit_in_add_only T\<close>
+    \<open>enc_weight_opt.cdcl_bnb_stgy S T\<close> and
+    struct: \<open>cdcl\<^sub>W_restart_mset.cdcl\<^sub>W_all_struct_inv (enc_weight_opt.abs_state S)\<close> and
+    dist: \<open>distinct_mset (normalize_clause `# learned_clss S)\<close>
+  shows \<open>distinct_mset (normalize_clause `# learned_clss T)\<close>
   using assms(1)
 proof (cases)
-  case (cdcl_conflict)
-  then show ?thesis
-    using lone ndec by (auto simp: lonely_lit_in_add_only_def
-    conflict.simps)
+  case cdcl_bnb_conflict
+  then show ?thesis using dist by (auto elim!: rulesE)
 next
-  case (cdcl_propagate)
-  then show ?thesis
-    using lone ndec by (auto simp: lonely_lit_in_add_only_def
-    propagate.simps)
+  case cdcl_bnb_propagate
+  then show ?thesis using dist by (auto elim!: rulesE)
 next
-  case (cdcl_improve)
-  then show ?thesis
-    using lone ndec by (auto simp: enc_weight_opt.improvep.simps
-      lonely_lit_in_add_only_def)
+  case cdcl_bnb_improve
+  then show ?thesis using dist by (auto elim!: enc_weight_opt.improveE)
 next
-  case (cdcl_conflict_opt0)
-  then show ?thesis
-    using lone ndec by (auto simp: conflict_opt0.simps
-      lonely_lit_in_add_only_def)
+  case cdcl_bnb_conflict_opt
+  then show ?thesis using dist by (auto elim!: enc_weight_opt.conflict_optE)
 next
-  case cdcl_simple_backtrack_conflict_opt
-  then show ?thesis
-    using lone ndec by (auto simp: lonely_lit_in_add_only_def
-      DECO_clause_def atms_of_def annotated_lit.is_decided_def
-      simple_backtrack_conflict_opt.simps lonely_not_decided_def)
-next
-  case cdcl_o'
+  case cdcl_bnb_other'
   then show ?thesis
   proof cases
     case decide
-    then show ?thesis
-    using lone ndec by (auto simp: lonely_lit_in_add_only_def
-      DECO_clause_def atms_of_def annotated_lit.is_decided_def
-      odecide.simps lonely_not_decided_def)
+    then show ?thesis using dist by (auto elim!: rulesE)
   next
     case bj
     then show ?thesis
     proof cases
       case skip
-      then show ?thesis
-        using lone ndec by (auto simp: lonely_lit_in_add_only_def
-          DECO_clause_def atms_of_def annotated_lit.is_decided_def
-          skip.simps lonely_not_decided_def)
-    next
-      case backtrack
-      then obtain D L K i M1 M2 D' where
-	conf: "conflicting S = Some (add_mset L D)" and
-	decomp: "(Decided K # M1, M2) \<in> set (get_all_ann_decomposition (trail S))" and
-	lev: "get_level (trail S) L = backtrack_lvl S" and
-	max: "get_level (trail S) L = get_maximum_level (trail S) (add_mset L D')" and
-	max_D: "get_maximum_level (trail S) D' \<equiv> i" and
-	lev_K: "get_level (trail S) K = Suc i" and
-	D'_D: \<open>D' \<subseteq># D\<close> and
-	NU_DL: \<open>clauses S + enc_weight_opt.conflicting_clss S \<Turnstile>pm add_mset L D'\<close> and
-	T: "T \<sim> cons_trail (Propagated L (add_mset L D'))
-		    (reduce_trail_to M1
-		      (add_learned_cls (add_mset L D')
-			(update_conflicting None S)))"
-	by (elim enc_weight_opt.obacktrackE) auto
-      show ?thesis
-        unfolding lonely_lit_in_add_only_def
-      proof (intro conjI allI impI)
-	fix K :: \<open>'v\<close> and C :: \<open>'v literal multiset\<close>
-	assume
-	  \<open>K \<in> \<Delta>\<Sigma>\<close> and
-	  \<open>C \<in># clauses T\<close> and
-	  \<open>K \<in> atms_of C\<close>
-(*	then show \<open>C \<in># additional_constraint K\<close>
-          using lone ndec T conf apply (auto simp: lonely_lit_in_add_only_def
-            DECO_clause_def atms_of_def annotated_lit.is_decided_def
-            enc_weight_opt.obacktrack.simps lonely_not_decided_def)
-	    sorry
-      next
-	fix K :: \<open>'v\<close>
-	assume
-	  \<open>K \<in> \<Delta>\<Sigma>\<close> and
-	  \<open>conflicting T \<noteq> None\<close> and
-	  \<open>K \<in> atms_of (the (conflicting T))\<close>
-	show \<open>the (conflicting T) \<in># additional_constraint K\<close> sorry
-      qed
+      then show ?thesis using dist by (auto elim!: rulesE)
     next
       case resolve
+      then show ?thesis using dist by (auto elim!: rulesE)
+    next
+      case backtrack
+      then obtain M1 M2 :: \<open>('v, 'v clause) ann_lits\<close> and K L :: \<open>'v literal\<close> and
+          D D' :: \<open>'v clause\<close> where
+	confl: \<open>conflicting S = Some (add_mset L D)\<close> and
+	\<open>(Decided K # M1, M2) \<in> set (get_all_ann_decomposition (trail S))\<close> and
+	\<open>get_maximum_level (trail S) (add_mset L D') = local.backtrack_lvl S\<close> and
+	\<open>get_level (trail S) L = local.backtrack_lvl S\<close> and
+	\<open>get_level (trail S) K = Suc (get_maximum_level (trail S) D')\<close> and
+	D'_D: \<open>D' \<subseteq># D\<close> and
+	\<open>set_mset (clauses S) \<union> set_mset (enc_weight_opt.conflicting_clss S) \<Turnstile>p
+	 add_mset L D'\<close> and
+	T: \<open>T \<sim>
+	   cons_trail (Propagated L (add_mset L D'))
+	    (reduce_trail_to M1
+	      (add_learned_cls (add_mset L D') (update_conflicting None S)))\<close>
+        by (auto simp: enc_weight_opt.obacktrack.simps)
+      have
+        tr_D: \<open>trail S \<Turnstile>as CNot (add_mset L D)\<close> and
+        \<open>distinct_mset (add_mset L D)\<close> and
+	\<open>cdcl\<^sub>W_restart_mset.cdcl\<^sub>W_M_level_inv (abs_state S)\<close>
+        using struct confl
+	unfolding cdcl\<^sub>W_restart_mset.cdcl\<^sub>W_all_struct_inv_def
+	  cdcl\<^sub>W_restart_mset.cdcl\<^sub>W_conflicting_def
+	  cdcl\<^sub>W_restart_mset.distinct_cdcl\<^sub>W_state_def
+	by auto
+      have tr_D': \<open>trail S \<Turnstile>as CNot (add_mset L D')\<close>
+        using D'_D tr_D
+	by (auto simp: true_annots_true_cls_def_iff_negation_in_model)
+      have \<open>-normalize_lit L2 \<in> lits_of_l (trail S) \<longleftrightarrow> -L2 \<in> lits_of_l (trail S)\<close>
+        if \<open>L2 \<in># D\<close>
+	for L2
+	using multi_member_split[OF that] tr_D
+	apply (cases L2)
+	apply (use that in auto)
+	oops
+(*
+	sorry
+      have False
+	if
+	  C: \<open>add_mset (normalize_lit L) (normalize_clause D') = normalize_clause C\<close> and
+	  \<open>C \<in># learned_clss S\<close>
+	for C
+      proof -
+        obtain L' C' where
+	  C_L'_C'[simp]: \<open>C = add_mset L' C'\<close> and
+	  \<open>normalize_clause C' = normalize_clause D'\<close> and
+	  [simp]: \<open>normalize_lit L' = normalize_lit L\<close>
+	  using C msed_map_invR[of \<open>normalize_lit\<close> C \<open>normalize_lit L\<close> \<open>normalize_clause D'\<close>]
+	  by auto
+	have \<open>trail S \<Turnstile>as CNot C'\<close>
+	  unfolding true_annots_true_cls_def_iff_negation_in_model
+	proof
+	  fix A
+	  assume \<open>A \<in># C'\<close>
+	  then obtain A' where
+	    \<open>A' \<in># D'\<close> and
+	    \<open>normalize_lit A' = normalize_lit A\<close>
+	    using \<open>normalize_clause C' = normalize_clause D'\<close>[symmetric]
+	    by (force dest!: msed_map_invR multi_member_split)
+	  then have \<open>- A' \<in> lits_of_l (trail S)\<close>
+	    using tr_D' by (auto dest: multi_member_split)
+	  then have \<open>-normalize_lit A' \<in> lits_of_l (trail S)\<close>
+	    apply (cases A')
+	    apply auto
+	    sorry
+	  then show \<open>- A \<in> lits_of_l (trail S)\<close>
+	    sorry
+	qed
+        show False sorry
+      qed
       then show ?thesis
-        using lone ndec by (auto simp: lonely_lit_in_add_only_def
-          DECO_clause_def atms_of_def annotated_lit.is_decided_def
-          resolve.simps lonely_not_decided_def)
+        using dist T
+        by (auto simp: enc_weight_opt.obacktrack.simps)
     qed
-    sorry
-  qed*)
-oops
+  qed
+qed
+*)
+
+end
 
 end
 
